logic bundles replaced with boolean

LeftistHeap.v
@@ -6,14 +6,6 @@ Notation ordType := (orderType tt).
 
 Open Scope order_scope.
 
-Module LeftistHeap.
-(*Leftist heaps are heap-ordered binary trees that satisfy the
-leftist property: the rank of any left child is at least as large as the rank of its
-right sibling. The rank of a node is defined to be the length of its right spine
-(i.e., the rightmost path from the node in question to an empty node). A simple
-consequence of the leftist property is that the right spine of any node is always
-the shortest path to an empty node.*)
-
 Lemma fst_true a b : true || a || b.
 Proof.
 by apply/orP; left.
@@ -32,41 +24,71 @@ by apply/orP; right.
 Qed.
 Hint Resolve trd_true : core.
 
+Lemma lt_le n : (0 < n)%N -> (n <= 0)%N = false.
+Proof.
+case H : (n <= 0)%N=> //.
+by move/leq_trans/(_ H).
+Qed.
 
+Lemma leq_1 : forall (a b : nat), (a <= b)%N -> (a.+1 <= b.+1)%N.
+Proof. by move=> a b H; ssrnatlia. Qed.
+
+
+Lemma nlt_gt : forall a b, (a <= b)%N = false -> (b < a)%N.
+Proof.
+move=> a b /neq0_lt0n. ssrnatlia.
+Qed.    
+
+Module leftistheap.
+(*Leftist heaps are heap-ordered binary trees that satisfy the
+leftist property: the rank of any left child is at least as large as the rank of its
+right sibling. The rank of a node is defined to be the length of its right spine
+(i.e., the rightmost path from the node in question to an empty node). A simple
+consequence of the leftist property is that the right spine of any node is always
+the shortest path to an empty node.*)
 
 Section LeftistDef.
-Variables (Elem : ordType).
+Variables (T: ordType).
 
 Hint Resolve lexx : core.
 
-Inductive Heap :=
-| E : Heap
-| T : nat -> Elem -> Heap -> Heap -> Heap.
+Inductive heap :=
+| Emp : heap
+| Node : nat -> T-> heap -> heap -> heap.
+
+
+Definition empty h :=
+if h is Emp then true else false.
+
+Theorem emptyP h : reflect (h = Emp) (empty h).
+Proof. case h; by constructor. Qed.
+
+Implicit Type h : heap.
 
 Definition LE x h : bool := 
-if h is T n y a b then (x <= y) else true.
+if h is Node n y a b then (x <= y) else true.
 
-Fixpoint HeapOrder h : bool :=
-if h is T n x tl tr then (LE x tl) && (LE x tr) && (HeapOrder tl) && (HeapOrder tr) else true.
+Fixpoint heap_ordered h : bool :=
+if h is Node n x tl tr then (LE x tl) && (LE x tr) && (heap_ordered tl) && (heap_ordered tr) else true.
 
 
-Fixpoint rk (h : Heap) : nat := if h is T _ _ _ b then (rk b).+1 else O.
+Fixpoint rk h : nat := if h is Node _ _ _ b then (rk b).+1 else O.
 
-Fixpoint Rank_Rk h : bool :=
+Fixpoint rank_rk h : bool :=
 match h with
-| T n x tl tr => (n == (rk tr).+1) && (Rank_Rk tr) && (Rank_Rk tl)
-| E           => true
+| Node n x tl tr => (n == (rk tr).+1) && (rank_rk tl) && (rank_rk tr)
+| Emp           => true
 end.
   
 
-Fixpoint rank (H : Heap) : nat := if H is T r _ _ _ then r else O.
+Fixpoint rank h : nat := if h is Node r _ _ _ then r else O.
 
-Fixpoint Leftist_Inv h : bool :=
-if h is T n x tl tr then
-  (Leftist_Inv tl) && (Leftist_Inv tr) && (rank tr <= rank tl)%N
+Fixpoint leftist_inv h : bool :=
+if h is Node n x tl tr then
+  (rank tr <= rank tl)%N && (leftist_inv tl) && (leftist_inv tr)
 else true.
 
-Lemma rank_correct : forall H, Rank_Rk H -> rk H = rank H.
+Lemma rank_correct : forall h, rank_rk h -> rk h = rank h.
 Proof. by move=> [] //= n _ tl tr /andP[/andP[/eqP]]. Qed.
 
 Inductive side := r | l.
@@ -75,9 +97,9 @@ Definition spine := seq side.
 
 Fixpoint spine_in p h : bool :=
 match p, h with
-| r :: p, T _ _ _ tr => spine_in p tr
-| l :: p, T _ _ tl _ => spine_in p tl
-| [::],   E          => true
+| r :: p, Node _ _ _ tr => spine_in p tr
+| l :: p, Node _ _ tl _ => spine_in p tl
+| [::],   Emp          => true
 | _,      _          => false
 end.
 
@@ -88,43 +110,40 @@ match p with
 | [::]    => true
 end.
 
-Lemma Rigth_correct : forall x s, Right (x :: s) -> (x = r /\ Right s).
+Lemma rigth_correct : forall x s, Right (x :: s) -> ((x = r) * Right s).
 Proof. move=> [] //=. Qed.
 
 Lemma case_spine_in : forall side s n x tl tr, 
-spine_in (side :: s) (T n x tl tr) -> 
+spine_in (side :: s) (Node n x tl tr) -> 
 if side is r then spine_in s tr else spine_in s tl.
 Proof. move=> [] //=. Qed. 
 
-Definition Leftist_Rank_Inv (H : Heap) := Leftist_Inv H /\ Rank_Rk H.
+Definition leftist_rank_inv h := leftist_inv h && rank_rk h.
 
 
-Lemma case_Leftist_Rank_Inv_r: forall n x tl tr,
-Leftist_Rank_Inv (T n x tl tr) -> Leftist_Rank_Inv tr.
+Lemma case_leftist_rank_inv_r n x tl tr :
+leftist_rank_inv (Node n x tl tr) -> leftist_rank_inv tr.
 Proof.
-by move=> n x tl tr [] /= /andP[/andP[_ Ltr _ /andP[/andP[]]]].
+by rewrite /leftist_rank_inv /= => /andP[/andP[/andP[_ _ -> /andP[_]]]].
 Qed.
 
-Lemma case_Leftist_Rank_Inv_rl: forall n x tl tr,
-Leftist_Rank_Inv (T n x tl tr) -> 
-Leftist_Rank_Inv tr /\ Leftist_Rank_Inv tl /\ (rank tr <= rank tl)%N.
-Proof. by move=> n x tl tr [/= /andP[/andP[LIl LIr R /andP[/andP[]]]]]. Qed.
-
-Lemma case_Rank_Rk n y h1 h2 : 
-Rank_Rk (T n y h1 h2) -> (n = (rk h2).+1) /\ (Rank_Rk h1) /\ (Rank_Rk h2).
-Proof. by move=> /= /andP[/andP[/eqP]]. Qed.
-
-Lemma case_HeapOrder n y h1 h2 : 
-HeapOrder (T n y h1 h2) ->
-LE y h1 /\ LE y h2 /\ (HeapOrder h1) /\ (HeapOrder h2).
-Proof. by move=> /= /andP[/andP[/andP[]]]. Qed.      
-
-
-Lemma lt_le n : (0 < n)%N -> (n <= 0)%N = false.
+Lemma case_leftist_rank_inv_rl n x tl tr:
+leftist_rank_inv (Node n x tl tr) -> 
+leftist_rank_inv tr && leftist_rank_inv tl && (rank tr <= rank tl)%N.
 Proof.
-case H : (n <= 0)%N=> //.
-by move/leq_trans/(_ H).
+rewrite /leftist_rank_inv=> /andP[] /=;
+by move=> /andP[/andP[->->->/andP[/andP[_ ->->]]]].
 Qed.
+
+Lemma case_rank_rk n y h1 h2 : 
+rank_rk (Node n y h1 h2) -> (n == (rk h2).+1) && (rank_rk h1) && (rank_rk h2).
+Proof. by []. Qed.
+
+Lemma case_heap_ordered n y h1 h2 : 
+heap_ordered (Node n y h1 h2) ->
+LE y h1 && LE y h2 && (heap_ordered h1) && (heap_ordered h2).
+Proof. by []. Qed.      
+
 
 Ltac merge_cases := match goal with 
 | H : (?x <= ?y) = true |- _ => move: (H)=> /= ->; rewrite ?H
@@ -139,95 +158,88 @@ Qed.
 
 Ltac swapg := apply swap_tact.
 
-Lemma case_Leftist_inv n y h1 h2 : 
-Leftist_Inv (T n y h1 h2) -> ((rank h2 <= rank h1)%N /\ Leftist_Inv h1 /\ Leftist_Inv h2).
-Proof. by move=> /= /andP[/andP[]]. Qed.
+Lemma case_leftist_inv n y h1 h2 : 
+leftist_inv (Node n y h1 h2) -> ((rank h2 <= rank h1)%N && leftist_inv h1 && leftist_inv h2).
+Proof. by []. Qed.
 
-Lemma leq_1 : forall (a b : nat), (a <= b)%N -> (a.+1 <= b.+1)%N.
-Proof. by move=> a b H; ssrnatlia. Qed.
-
-Lemma Right_spine_ex : forall H, exists s, Right s /\ spine_in s H.
+Lemma right_spine_ex : forall h, exists s, Right s && spine_in s h.
 Proof.
-elim=> [|n s hl _ hr [] s' [] IHHR IHHS].
+elim=> [|n s hl _ hr [] s'].
 - by exists nil.
 by exists (r :: s').
 Qed.
 
-Lemma length_right_spine : forall H s, 
-Leftist_Rank_Inv H -> Right s -> spine_in s H ->
-length s = rank H.
+Lemma length_right_spine : forall h s, 
+leftist_rank_inv h -> Right s -> spine_in s h ->
+length s = rank h.
 Proof.
-move=> h s [] _ RC; move: (RC)=> /rank_correct <-.
+move=> h s /andP [] _ RC; move: (RC)=> /rank_correct <-.
 elim: h s RC=> 
 [[|[]]|n x tl IHhl tr IHtr [_ _|[s /= /andP[/andP[_ RRl RRr]] |]]] //= R S.
 apply/eqnP=> /=. apply/eqP. by apply: IHtr.
 Qed.
 
-Lemma spine_in_E s : spine_in s E -> s = [::].
+Lemma spine_in_E s : spine_in s Emp -> s = [::].
 Proof. by case: s=> [|[]] //=. Qed.
 
 Theorem rigth_spine_shortest : 
-forall H s1 s2, Right s1 -> Leftist_Rank_Inv H -> spine_in s1 H -> spine_in s2 H ->
+forall H s1 s2, Right s1 -> leftist_rank_inv H -> spine_in s1 H -> spine_in s2 H ->
 (length s1 <= length s2)%nat.
 Proof. 
 elim=>
 [s1 s2 _ _ /spine_in_E->|
 n x tl IHtl tr IHtr [//|
-a s1 [/Rigth_correct [] -> _ _ _ |[]
-s2 /Rigth_correct [] ->]]] //= => [Rs1 /case_Leftist_Rank_Inv_r LI|
-Rs1 /case_Leftist_Rank_Inv_rl [] LI1 [] LI2 LE]=> SI1 SI2.
+a s1 [/rigth_correct [] -> _ _ _ |[]
+s2 /rigth_correct [] ->]]] //= => [Rs1 /case_leftist_rank_inv_r LI|
+Rs1 /case_leftist_rank_inv_rl /andP[/andP[LI1 LI2 LE]]] => SI1 SI2.
 - apply: leq_1; apply IHtr=> //.
 rewrite (length_right_spine tr s1) //.
-case: (Right_spine_ex tl)=> s [] Rs SIstl.
+case: (right_spine_ex tl)=> s /andP [] Rs SIstl.
 suffices: (rank tl <= length s2)%N. ssrnatlia.
 rewrite -(length_right_spine tl s) //.
 by apply: IHtl.
 Qed.
 
-Definition makeT (x : Elem) (a b : Heap) : Heap :=
-if (rank b <= rank a)%N then T (rank b).+1 x a b else T (rank a).+1 x b a.
-
-Lemma nlt_gt : forall a b, (a <= b)%N = false -> (b < a)%N.
-Proof.
-move=> a b /neq0_lt0n. ssrnatlia.
-Qed.    
+Definition makeT (x : T) (a b : heap) : heap :=
+if (rank b <= rank a)%N then Node (rank b).+1 x a b else Node (rank a).+1 x b a.
 
 Lemma makeT_preserves_LI_inv : forall x tl tr,
-Leftist_Inv tl -> Leftist_Inv tr ->
-Leftist_Inv (makeT x tl tr).
+leftist_inv tl -> leftist_inv tr ->
+leftist_inv (makeT x tl tr).
 Proof.
-  rewrite /makeT=> x tl tr; case H : (rank tr <= rank tl)%N=> /=->->//=.
-  move: H=> /nlt_gt; by ssrnatlia.
+  rewrite /makeT=> x tl tr; case H : (rank tr <= rank tl)%N=> /=->->.
+  - by rewrite H.
+  move: H=> /nlt_gt H. apply/andP; split=> //; apply/andP; split=>//. by ssrnatlia.
 Qed.
 
 Lemma makeT_preserves_rk_inv x tl tr :
-Rank_Rk tl -> Rank_Rk tr ->
-Rank_Rk (makeT x tl tr).
+rank_rk tl -> rank_rk tr ->
+rank_rk (makeT x tl tr).
 Proof.
 move=> Rl Rr; rewrite /makeT -!(rank_correct _ Rl) -!(rank_correct _ Rr).
 by case H : (rk tr <= rk tl)%N=> /=; rewrite Rl Rr eq_refl.
 Qed.
 
 Lemma makeT_peserves_HO_inv x tl tr :
-HeapOrder tl -> HeapOrder tr ->
+heap_ordered tl -> heap_ordered tr ->
 LE x tl -> LE x tr ->
-HeapOrder (makeT x tl tr).
+heap_ordered (makeT x tl tr).
 Proof.
 by rewrite /makeT; case H : (rank tr <= rank tl)%N=> /=->->->->.
 Qed.
 
-Fixpoint member x (h : Heap) :=
-if h is T _ y a b then (x == y) || (member x a) || (member x b) else false.
+Fixpoint member x h :=
+if h is Node _ y a b then (x == y) || (member x a) || (member x b) else false.
 
 Notation "x ? h" := (member x h) (at level 0).
 
-Definition LeftistHeap (h : Heap) :=
-Leftist_Inv h /\ Rank_Rk h /\ HeapOrder h.
+Definition leftistheap h :=
+leftist_inv h && rank_rk h && heap_ordered h.
 
 Fixpoint merge a :=
-if a is T n x a1 b1 then
+if a is Node n x a1 b1 then
 let fix merge_a b :=
-  if b is T m y a2 b2 then
+  if b is Node m y a2 b2 then
     if x <= y then 
       makeT x a1 (merge b1 b)
     else
@@ -238,26 +250,26 @@ else id.
 
 Arguments merge !tl !tr : rename.
 
-Lemma merge_E_h: forall h, merge E h = h.
+Lemma merge_E_h: forall h, merge Emp h = h.
 Proof.  by case. Qed.
 Hint Rewrite merge_E_h.
 
-Lemma merge_h_E: forall h, merge h E = h.
+Lemma merge_h_E: forall h, merge h Emp = h.
 Proof. by case. Qed.
 Hint Rewrite merge_h_E.
 
-Lemma Rank_Rk_r n x tl tr:
-Rank_Rk (T n x tl tr) -> Rank_Rk tr.
+Lemma rank_rk_r n x tl tr:
+rank_rk (Node n x tl tr) -> rank_rk tr.
 Proof. by move=> /andP[/andP[]]. Qed.
 
-Lemma Rank_Rk_l n x tl tr :
-Rank_Rk (T n x tl tr) -> Rank_Rk tl.
+Lemma rank_rk_l n x tl tr :
+rank_rk (Node n x tl tr) -> rank_rk tl.
 Proof. by move=> /andP[/andP[]]. Qed.
 
 Lemma merge_a nl nr x y tll tlr trr trl :
 (x <= y) = false -> 
-merge (T nl x tll tlr) (T nr y trl trr) = 
-makeT y trl (merge  (T nl x tll tlr) trr).
+merge (Node nl x tll tlr) (Node nr y trl trr) = 
+makeT y trl (merge  (Node nl x tll tlr) trr).
 Proof.
 move=> /= ->.
 by elim: trr.
@@ -265,27 +277,27 @@ Qed.
 
 Hint Rewrite merge_a.
 Lemma merge_preserve_rk_inv : forall h1 h2,
-Rank_Rk h1 -> Rank_Rk h2 -> Rank_Rk (merge h1 h2) .
+rank_rk h1 -> rank_rk h2 -> rank_rk (merge h1 h2) .
 Proof.
 elim=> [//| nl x tll IHhl tlr IHhr].
 elim=> [|nr y trl IH'hl trr IH'hr] //.
 case H : (x <= y)=> H1 H2; merge_cases;
-move: (H1) (H2) => /case_Rank_Rk [_ [HH1 HH2]] /case_Rank_Rk [_ [HH3 HH4]];
-apply makeT_preserves_rk_inv=> //.
-- by apply IHhr.
-by apply IH'hr.
+move: (H1) (H2) => /case_rank_rk /andP[/andP[_ HH1 HH2]] /case_rank_rk /andP[/andP[_ HH3 HH4]];
+apply: makeT_preserves_rk_inv=> //.
+- by apply: IHhr.
+by apply: IH'hr.
 Qed.
 
-Lemma case_HeapOrder_l n x tl tr :
-HeapOrder (T n x tl tr) -> (HeapOrder tl /\ LE x tl).
-Proof. by move=> /andP[/andP[/andP[]]]. Qed.
+Lemma case_heap_ordered_l n x tl tr :
+heap_ordered (Node n x tl tr) -> (heap_ordered tl && LE x tl).
+Proof. by move=> /= /andP[/andP[/andP[-> _ ->]]]. Qed.
 
-Lemma case_HeapOrder_r n x tl tr :
-HeapOrder (T n x tl tr) -> (HeapOrder tr /\ LE x tr).
-Proof. by move=> /andP[/andP[/andP[]]]. Qed.
+Lemma case_heap_ordered_r n x tl tr :
+heap_ordered (Node n x tl tr) -> (heap_ordered tr && LE x tr).
+Proof. by move=> /= /andP[/andP[/andP[_ -> _ ->]]]. Qed.
 
 Lemma case_LE x y n tr tl :
-LE x (T n y tl tr) -> x <= y.
+LE x (Node n y tl tr) -> x <= y.
 Proof. by []. Qed.
 
 Ltac makeT_cases := match goal with
@@ -300,18 +312,18 @@ Proof.
 elim=> [//| nl x tll IHhl tlr IHhr].
 elim=> [|nr y trl IH'hl trr IH'hr x' /case_LE HH1 /case_LE HH2] //.
 by merge_casesxy x y; 
-[makeT_casesxy (rank (merge tlr (T nr y trl trr))) (rank tll)|
-  makeT_casesxy (rank (merge (T nl x tll tlr) trr)) (rank trl)].
+[makeT_casesxy (rank (merge tlr (Node nr y trl trr))) (rank tll)|
+  makeT_casesxy (rank (merge (Node nl x tll tlr) trr)) (rank trl)].
 Qed.
 
 Lemma merge_preserve_HO_inv : forall h1 h2,
-HeapOrder h1 -> HeapOrder h2 -> HeapOrder (merge h1 h2).
+heap_ordered h1 -> heap_ordered h2 -> heap_ordered (merge h1 h2).
 Proof.
 elim=> [//| nl x tll IHhl tlr IHhr].
 elim=> [|nr y trl IH'hl trr IH'hr H1 H2] //.
 move : (H1) (H2)=>
-        /case_HeapOrder [L1 [L2[HH1 HH2]]]
-        /case_HeapOrder [L'1 [L'2[HH'1 HH'2]]] //;
+        /case_heap_ordered /andP[/andP[/andP[L1 L2 HH1 HH2]]]
+        /case_heap_ordered /andP[/andP[/andP[L'1 L'2 HH'1 HH'2]]] //;
 merge_casesxy x y; apply makeT_peserves_HO_inv=> //.
 1 : apply: IHhr=> //.
 2 : apply: IH'hr=> //.
@@ -320,270 +332,224 @@ move: (negbT H).
 by rewrite -ltNge lt_def=> /andP[_ ->].
 Qed.
 
-Lemma case_Leftist_Inv_l n x tl tr : Leftist_Inv (T n x tl tr) -> Leftist_Inv tl.
+Lemma case_leftist_inv_l n x tl tr : leftist_inv (Node n x tl tr) -> leftist_inv tl.
 Proof. by move=> /andP[/andP[]].  Qed.
 
-Lemma case_Leftist_Inv_r n x tl tr : Leftist_Inv (T n x tl tr) -> Leftist_Inv tr.
+Lemma case_leftist_inv_r n x tl tr : leftist_inv (Node n x tl tr) -> leftist_inv tr.
 Proof. by move=> /andP[/andP[]].  Qed.
 
 Lemma merge_preserve_LI_inv : forall h1 h2,
-Leftist_Inv h1 -> Leftist_Inv h2 -> Leftist_Inv (merge h1 h2).
+leftist_inv h1 -> leftist_inv h2 -> leftist_inv (merge h1 h2).
 Proof.
 elim=> [//| nl x tll IHhl tlr IHhr].
 elim=> [|nr y trl IH'hl trr IH'hr H1 H2] //.
-move : (H1) (H2) => /case_Leftist_inv [_ [HH1 HH2]] /case_Leftist_inv [_ [HH'1 HH'2]].
+move : (H1) (H2) =>  /andP[/andP[_ HH1 HH2]] /andP[/andP[_ HH'1 HH'2]].
 merge_casesxy x y; apply: makeT_preserves_LI_inv=> //.
 - by apply: IHhr.
 by apply: IH'hr.
 Qed.    
 
 Theorem merge_preserve_LH h1 h2 :
-LeftistHeap h1 -> LeftistHeap h2 -> LeftistHeap (merge h1 h2).
+leftistheap h1 -> leftistheap h2 -> leftistheap (merge h1 h2).
 Proof.
-move=> [LI1 [RR1 HO1]] [LI2 [RR2 HO2]]; split.
+move=> /andP[/andP[LI1 RR1 HO1]] /andP[/andP[LI2 RR2 HO2]]; apply/andP; split.
+- apply/andP; split.
 - by apply: merge_preserve_LI_inv.
-- split.
 - by apply: merge_preserve_rk_inv.
 by apply: merge_preserve_HO_inv. 
 Qed.
 
 Lemma case_member : forall x y n tl tr,
-x ? (T n y tl tr) <-> (x = y) \/ (x ? tl) \/ (x ? tr).
-Proof.
-split.
-- move=> /orP[/orP[/eqP|]|]; by [left|right; left|right; right].
-case=> [->|[]H] /=; apply/orP.
-- by left; apply/orP; left.
-- by left; apply/orP; right.
-by right.
-Qed.
+x ? (Node n y tl tr) <-> (x == y) || (x ? tl) || (x ? tr).
+Proof. by []. Qed.
 
 Lemma makeT_spec h1 h2 x y :
-x ? (makeT y h1 h2) <-> (x = y) \/ (x ? h1) \/ (x ? h2).
+x ? (makeT y h1 h2) = ((x == y) || (x ? h1) || (x ? h2)).
 Proof.
 makeT_casesxy (rank h2) (rank h1).
-split => /case_member // [|[]].
-split=> [/case_member // [->|[]->]|[->/=|[]/=->]] //.
-- by left.
-- by right; right.
-- by right; left.
-by rewrite eq_refl.
+apply/idP/idP => /case_member // [|[]].
+by apply/idP/idP => /= /orP[/orP[]|]->.
 Qed.
 
-Theorem merge_spec : forall h1 h2 x,
-x ? (merge h1 h2) <-> (x ? h1) \/ (x ? h2).
+Theorem merge_spec  h1 h2 x :
+x ? (merge h1 h2) = ((x ? h1) || (x ? h2)).
 Proof.
-split.
+apply/idP/idP.
 - elim: h1 h2=> [h2|n y h1 IHh1 h2 IHh2].
-- rewrite merge_E_h=> H; by right.
-- elim=> [|m z h21 IHh21 h22 IHh22]; first by rewrite merge_h_E=> H; left.
-- merge_casesxy y z=> /makeT_spec [-> |[->|]].
-- by left; rewrite eq_refl.
-- by left.
-- move=> /IHh2 [->|]; [left|]=> //=; by right.
-1,2: by rewrite ?eq_refl; right.
-- move=> /IHh22 [/case_member [->|[]->]|->]; rewrite ?eq_refl.
-1-3: by left.
-- by right.
+- by rewrite merge_E_h=>->.
+- elim=> [|m z h21 IHh21 h22 IHh22]; first by rewrite merge_h_E=>->.
+- merge_casesxy y z; rewrite makeT_spec=> /orP[->|] //.
+- by move=> /IHh2 /= /orP[] ->.
+- move=> /IHh22 /= /orP[] -> //. apply/orP; by right.
 
-- elim: h1 h2=> [h [F|H]|n y h11 IHh1 h22 IHh2]; rewrite ?merge_E_h //.
-- elim=> [[] // F|m z h12 IHh12 h21 IHh21]; rewrite ?merge_h_E.
-merge_casesxy y z; case=> /orP[/orP[/eqP|]|]; rewrite makeT_spec.
-- by left.
-- by right; left.
-1-4: right; right; apply IHh2.
-- by left.
-1- 3: by right=> /=; rewrite H0 ?eq_refl.
-1-3, 6: right; right; apply IHh21=> /=; rewrite H0 ?eq_refl.
-1-3: by left.
-- by right.
-- by left.
-by right; left.
+- elim: h1 h2 => [h |n y h11 IHh1 h22 IHh2]; rewrite ?merge_E_h //.
+- elim=> [/orP [] //|m z h12 IHh12 h21 IHh21]; rewrite ?merge_h_E.
+merge_casesxy y z; move=> /orP[/orP[/orP[]|]|/orP[/orP[]|]]; rewrite makeT_spec.
+1,2: by move=>->.
+1-4: move=> HH; apply/orP; right=> /=; apply/ IHh2; rewrite /= HH //.
+1-3: apply/orP; by right.
+1-3,6: move=> HH; apply/orP; right=> /=; apply/ IHh21; rewrite /= HH //.
+- apply/orP; by left.
+1-2: by move=>->.
 Qed.
 
-Definition insert (x : Elem) (h : Heap) := 
-merge (T 1 x E E) h.
+Definition insert (x : T) (h : heap) := 
+merge (Node 1 x Emp Emp) h.
 
-Lemma rk_E : ((rk E).+1 = 1)%N.
+Lemma rk_E : ((rk Emp).+1 = 1)%N.
 Proof. by []. Qed.    
 
 Lemma insert_preserve_rk_inv : forall h x,
-Rank_Rk h -> Rank_Rk (insert x h).
+rank_rk h -> rank_rk (insert x h).
 Proof.
 by move=> h x Rh; apply merge_preserve_rk_inv.
 Qed.
 
 Lemma insert_preserve_HO_inv : forall h x,
-HeapOrder h -> HeapOrder (insert x h).
+heap_ordered h -> heap_ordered (insert x h).
 Proof.
 by move=> h x Rh; apply merge_preserve_HO_inv.
 Qed.
 
 Lemma insert_preserve_LI_inv : forall h x,
-Leftist_Inv h -> Leftist_Inv (insert x h).
+leftist_inv h -> leftist_inv (insert x h).
 Proof.
 by move=> h x Rh; apply merge_preserve_LI_inv.
 Qed.
 
 Theorem insert_preserve_LH : forall h x,
-LeftistHeap h -> LeftistHeap (insert x h).
+leftistheap h -> leftistheap (insert x h).
 Proof.
 by move=> h x Rh; apply merge_preserve_LH.
 Qed.
 
-Lemma x_Ty x y : (x) ? (T 1 y E E) <-> (x = y).
-Proof.
-by split=> /= [/orP[/orP[/eqP|]|]|->]; rewrite ?eq_refl.
-Qed.
 
 Theorem insert_correct h x y :
-x ? (insert y h) <-> (x = y) \/ (x ? h).
+x ? (insert y h) = ((x == y) || (x ? h)).
 Proof.
-by rewrite merge_spec x_Ty.
+rewrite merge_spec /=; case (x == y); by case (x ? h).
 Qed.
 
-Definition findMin (h : Heap) := 
-if h is T _ x _ _ then Some x else None.
+Definition findmin h := 
+if h is Node _ x _ _ then Some x else None.
 
-Theorem findMin_correct1 : forall h,
-None = findMin h <-> h = E.
+Theorem findmin_correct1 : forall h,
+None = findmin h <-> h = Emp.
 Proof. split=> [|-> //]. by case : h. Qed.
 
 Lemma LE_correct : forall h x y,
-HeapOrder h -> x ? h -> LE y h -> y <= x.
+heap_ordered h -> x ? h -> LE y h -> y <= x.
 Proof.
-elim=> [x y _ H| n x h1 IHh1 h2 IHh2 x' y' HO /case_member 
-[-> /case_LE //|[H|H] /case_LE]]//.
-move: HO=> /case_HeapOrder_l [] /IHh1 H1 /(H1 x' x H) H2 H3.
-2: move: HO=> /case_HeapOrder_r [] /IHh2 H1 /(H1 x' x H) H2 H3.
-all: move: H3 H2; apply: le_trans.
+elim=> [x y _ H| n x h1 IHh1 h2 IHh2 x' y' /= /andP[/andP[/andP[L1 L2 H1 H2]]]] //
+ /orP[/orP[/eqP ->|/(IHh1 _ _ H1)/(_ L1)]|/(IHh2 _ _ H2)/(_ L2)] //; swapg; exact: le_trans.
 Qed.
 
-Theorem findMin_correct2 : forall h, HeapOrder h ->
-forall z, Some z = findMin h -> forall x, x ? h -> z <= x.
+Theorem findmin_correct2 : forall h, heap_ordered h ->
+forall z, Some z = findmin h -> forall x, x ? h -> z <= x.
 Proof.
-case=> [//| n x h1 h2 HO z /= [->] y /(case_member _ _ n)[-> //|[H|H]]].
-- by move: HO=> /case_HeapOrder_l [] /LE_correct - /(_ _ x H).
-- by move: HO=> /case_HeapOrder_r [] /LE_correct - /(_ _ x H).
+case=> [//| n x h1 h2 HO z /= [->] y /orP[/orP[/eqP ->|]|]] // H. 
+- by move: HO=> /case_heap_ordered_l /andP[/LE_correct - /(_ _ x H)].
+by move: HO=> /case_heap_ordered_r /andP[/LE_correct - /(_ _ x H)].
 Qed.
 
-Lemma findMin_cases : forall h, (exists x, Some x = findMin h) \/ (h = E).
+Lemma findmin_cases : forall h, (exists x, Some x = findmin h) \/ (h = Emp).
 Proof.
 case=> [|n z h1 h2 /=]; first by right.
 by left; exists z.
 Qed.
 
-Theorem findMin_LE_correct : forall x h,
-HeapOrder h ->
-(x ? h /\ LE x h) <-> (Some x = findMin h).
+Theorem findmin_LE_correct : forall x h,
+heap_ordered h ->
+(x ? h && LE x h) <-> (Some x = findmin h).
 Proof.
-split=> [[]|]; move: h H=> [] //.
-- move=> n y h1 h2 H /case_member [-> //|[HH|HH] /case_LE XY];
-  suffices: x = y=> [-> //|]; move: H.
-- move=> /case_HeapOrder_l [] /LE_correct L /(L _ _ HH) YX.
-apply: le_anti. by apply/andP.
-- move=> /case_HeapOrder_r [] /LE_correct L /(L _ _ HH) YX.
-apply: le_anti. by apply/andP.
-move=> n s h1 h2 HO [] ->; split=> /=. 
+split=> [/andP[]|]; move: h H=> [] //.
+- move=> n y h1 h2 /= /andP[/andP[/andP[L1 L2 H1 H2]]]
+  /orP[/orP[/eqP-> //|/(LE_correct _ _ _ H1)/(_ L1)]|/(LE_correct _ _ _ H2)/(_ L2)] XY YX;
+  suffices: x = y=> [-> //|]; apply: le_anti; rewrite XY YX //.
+move=> n s h1 h2 HO [] ->; apply/andP; split=> /=. 
 - by rewrite eq_refl.
 by apply lexx.
 Qed.
 
-Definition deleteMin (h : Heap) :=
-if h is T _ _ a b then merge a b else E.
+Definition deletemin h :=
+if h is Node _ _ a b then merge a b else Emp.
 
-Lemma Rank_Rk_eq n x h1 h2 :
-Rank_Rk (T n x h1 h2) -> n = (rk h2).+1.
+Lemma rank_rk_eq n x h1 h2 :
+rank_rk (Node n x h1 h2) -> n = (rk h2).+1.
 Proof. by move=> /andP[/andP[/eqP]]. Qed.
 
 Lemma case_LE' x y h1 h2 n :
-LE x (T n y h1 h2) -> ((x <= y) = true).
+LE x (Node n y h1 h2) -> ((x <= y) = true).
 Proof. by move=> /= ->. Qed.
 
 Lemma rk1 : forall m y h1 h2,
-(1 <= rk (T m y h1 h2))%N.
+(1 <= rk (Node m y h1 h2))%N.
 Proof. move=> m y h1 h2 /=. ssrnatlia. Qed.
 
 Lemma rank1 : forall m y h1 h2,
-Rank_Rk (T m y h1 h2) -> (1 <= rank (T m y h1 h2))%N.
+rank_rk (Node m y h1 h2) -> (1 <= rank (Node m y h1 h2))%N.
 Proof. move=> m y h1 h2 /rank_correct <-. by apply rk1. Qed.
 
-Lemma rk0: rk E = 0.
+Lemma rk0: rk Emp = 0.
 Proof. by []. Qed.
 
-Lemma rank0: rank E = 0.
+Lemma rank0: rank Emp = 0.
 Proof. by []. Qed.
 
-Lemma LI_exfalso n x m y h1 h2 :
-LeftistHeap (T n x E (T m y h1 h2)) -> False.
+Lemma case_leftistheap_l n x h1 h2 :
+leftistheap (Node n x h1 h2) -> leftistheap h1.
 Proof.
-move=> [/= /andP[/andP[/andP[]]]] LI1 LI2 rr M0 [/andP[/andP[]]] _
-  /andP[/andP[/eqP M RR1 RR2 _]] _.
-by move : M M0=>-> //.
+by rewrite /leftistheap => /andP[/andP[/case_leftist_inv_l-> /rank_rk_l-> /case_heap_ordered_l /andP[-> _]]].
 Qed.
 
-Lemma case_LeftistHeap_l n x h1 h2 :
-LeftistHeap (T n x h1 h2) -> LeftistHeap h1.
-Proof.
-move=> [/case_Leftist_Inv_l LI [/Rank_Rk_l RR /case_HeapOrder_l [HO _]]].
-split=> [//|]; by split.
-Qed.
-
-Lemma case_LeftistHeap_r n x h1 h2 :
-LeftistHeap (T n x h1 h2) -> LeftistHeap h2.
+Lemma case_leftistheap_r n x h1 h2 :
+leftistheap (Node n x h1 h2) -> leftistheap h2.
 Proof. 
-move=> [/case_Leftist_Inv_r LI2 [/Rank_Rk_r RR /case_HeapOrder_r [HO _]]].
-split=> [//|]; by split.
+by rewrite /leftistheap => /andP[/andP[/case_leftist_inv_r-> /rank_rk_r-> /case_heap_ordered_r /andP[-> _]]].
 Qed.
 
-Lemma deleMin_preserve_rk_inv : forall h, 
-Rank_Rk h -> Rank_Rk (deleteMin h).
+Lemma deletemin_preserve_rk_inv : forall h, 
+rank_rk h -> rank_rk (deletemin h).
 Proof.
 by case=> //=n x h1 h2 H; apply merge_preserve_rk_inv; move: H=> /andP[/andP[]].
 Qed.
 
-Lemma deleMin_preserve_HO_inv : forall h, 
-HeapOrder h -> HeapOrder (deleteMin h).
+Lemma deletemin_preserve_HO_inv : forall h, 
+heap_ordered h -> heap_ordered (deletemin h).
 Proof.
 by case=> //=n x h1 h2 H; apply merge_preserve_HO_inv; move: H=> /andP[/andP[]].
 Qed.
 
-Lemma deleMin_preserve_LI_inv : forall h, 
-Leftist_Inv h -> Leftist_Inv (deleteMin h).
+Lemma deletemin_preserve_LI_inv : forall h, 
+leftist_inv h -> leftist_inv (deletemin h).
 Proof.
 by case=> //=n x h1 h2 H; apply merge_preserve_LI_inv; move: H=> /andP[/andP[]].
 Qed.
 
-Lemma deleMin_correct : forall h, 
-LeftistHeap h -> LeftistHeap (deleteMin h).
+Lemma deletemin_correct : forall h, 
+leftistheap h -> leftistheap (deletemin h).
 Proof.
 case=> //=n x h1 h2 H; apply merge_preserve_LH; move: H.
-- by move/case_LeftistHeap_l.
-by move/case_LeftistHeap_r.
+- by move/case_leftistheap_l.
+by move/case_leftistheap_r.
 Qed.
 
-Theorem deleteMin_spec : forall h x y,
-Some x = findMin h -> (y ? (insert x (deleteMin h))) <-> y ? h.
+Theorem deletemin_spec : forall h x y,
+Some x = findmin h -> (y ? (insert x (deletemin h))) = y ? h.
 Proof.
-case=> [//=|n x h1 h2 y z [->]];
-by rewrite insert_correct /= merge_spec case_member.
+case=> [//=|n x h1 h2 y z [->]].
+by rewrite insert_correct /deletemin merge_spec //= orbA.
 Qed.
 
-Definition isEmpty (h : Heap) :=
-if h is E then true else false.
-
-Theorem emptyP h : reflect (h = E) (isEmpty h).
-Proof. by case h; constructor. Qed.
-
-Fixpoint insert' (x : Elem) (h : Heap) :=
-if h is T n y a b then
-let h' := T n y a b in 
+Fixpoint insert' (x : T) (h : heap) :=
+if h is Node n y a b then
+let h' := Node n y a b in 
   if x <= y then
-    T 1 x h' E
+    Node 1 x h' Emp
   else makeT y a (insert' x b)
-else T 1 x E E.
+else Node 1 x Emp Emp.
 
-Theorem insertE x h : Rank_Rk h -> Leftist_Inv h -> insert' x h = insert x h.
+Theorem insertE x h : rank_rk h -> leftist_inv h -> insert' x h = insert x h.
 Proof.
 rewrite /insert.
 elim h=> [//|n y h1 IHh1 h2 IHh2 RR]; move : RR (RR)=> /rank1.
@@ -593,41 +559,41 @@ by rewrite IHh2.
 Qed.
 
 End LeftistDef.
-End LeftistHeap.
-Module WBLeftistHeap.
+End leftistheap.
+Module WBleftistheap.
 (*Weight-biased leftist heaps are an al-
 ternative to leftist heaps that replace the leftist property with the weight-biased
 leftist property: the size of any left child is at least as large as the size of its
 right sibling.*)
 Section WBLeftistDef.
-Variables (Elem : ordType).
+Variables (T: ordType).
 
-Inductive Heap :=
-| E : Heap
-| T : nat -> Elem -> Heap -> Heap -> Heap.
+Inductive heap :=
+| Emp : heap
+| Node : nat -> T-> heap -> heap -> heap.
 Print negbT.
-Fixpoint rank (H : Heap) : nat :=
-if H is T r _ _ _ then r else O.
+Fixpoint rank (H : heap) : nat :=
+if H is Node r _ _ _ then r else O.
 
-Definition makeT (x : Elem) (a b : Heap) : Heap :=
+Definition makeT (x : T) (a b : heap) : heap :=
 if rank a >= rank b then 
-T ((rank b) + (rank a) + 1) x a b
-else T ((rank b) + (rank a) + 1) x b a.
+Node ((rank b) + (rank a) + 1) x a b
+else Node ((rank b) + (rank a) + 1) x b a.
 
-Fixpoint size (h : Heap) : nat :=
-if h is T _ _ a b then (size b) + (size a) + 1 else O.
+Fixpoint size (h : heap) : nat :=
+if h is Node _ _ a b then (size b) + (size a) + 1 else O.
 
-Definition isEmpty (h : Heap) :=
-if h is E then true else false.
+Definition isEmpty (h : heap) :=
+if h is Emp then true else false.
 
 
-Program Fixpoint merge (a b : Heap) {measure (size a + size b)} : Heap :=
+Program Fixpoint merge (a b : heap) {measure (size a + size b)} : heap :=
 match a, b with
-| h, E => h
-| E, h => h
-| T n x a1 b1, T m y a2 b2 =>
-let h1 := T n x a1 b1 in
-let h2 := T m y a2 b2 in
+| h, Emp => h
+| Emp, h => h
+| Node n x a1 b1, Node m y a2 b2 =>
+let h1 := Node n x a1 b1 in
+let h2 := Node m y a2 b2 in
 if leq x y then
   makeT x a1 (merge b1 h2)
 else
@@ -643,30 +609,30 @@ move=> /=;
 rewrite -!plusE; lia.
 Qed.
 
-Definition insert (x : Elem) (h : Heap) := 
-        merge (T 1 x E E) h.
+Definition insert (x : T) (h : heap) := 
+        merge (Node 1 x Emp Emp) h.
 
-Definition findMin (h : Heap) := 
-if h is T _ x _ _ then Some x else None.
+Definition findmin (h : heap) := 
+if h is Node _ x _ _ then Some x else None.
 
-Definition deleteMin (h : Heap) :=
-if h is T _ _ a b then merge a b else E.
+Definition deletemin (h : heap) :=
+if h is Node _ _ a b then merge a b else Emp.
 
-Program Fixpoint merge' (a b : Heap) {measure (size a + size b)} : Heap :=
+Program Fixpoint merge' (a b : heap) {measure (size a + size b)} : heap :=
 match a, b with
-| h, E => h
-| E, h => h
-| T w1 x a1 b1, T w2 y a2 b2 =>
-let h1 := T w1 x a1 b1 in
-let h2 := T w2 y a2 b2 in
+| h, Emp => h
+| Emp, h => h
+| Node w1 x a1 b1, Node w2 y a2 b2 =>
+let h1 := Node w1 x a1 b1 in
+let h2 := Node w2 y a2 b2 in
 if leq x y then
   if size a1 >= (size b1) + w2 then 
-    T (w1 + w2) x a1 (merge' b1 h2)
-  else T (w1 + w2) x (merge' b1 h2) a1
+    Node (w1 + w2) x a1 (merge' b1 h2)
+  else Node (w1 + w2) x (merge' b1 h2) a1
 else
   if size a2 >= w1 + size b2 then
-    T (w1 + w2) y a2 (merge' h1 b2)
-  else T (w1 + w2) y (merge' h1 b2) a2
+    Node (w1 + w2) y a2 (merge' h1 b2)
+  else Node (w1 + w2) y (merge' h1 b2) a2
 end.
 Next Obligation.
 move=> /=;
@@ -686,4 +652,4 @@ rewrite -!plusE; lia.
 Qed.
 
 End WBLeftistDef.
-End WBLeftistHeap.
+End WBleftistheap.
